Bachmair_Ganzinger/Multiset_Even_More.thy
@@ -141,7 +141,46 @@ qed
 theorem "\<forall>i < length xs. P (xs ! i) \<Longrightarrow> \<forall>x \<in> set xs. P x"
   using in_mset_conv_nth[of _ xs] by auto
     
-    
-    
-    
+
+
+
+lemma all_the_same: "\<forall>x \<in># X. x = y \<Longrightarrow> card (set_mset X) \<le> Suc 0"
+  by (metis card.empty card.insert card_mono finite.intros(1) finite_insert le_SucI singletonI subsetI)
+
+
+thm "sum_mset.remove"
+
+lemma Melem_subseteq_Union_mset[simp]:
+  assumes "x \<in># T"
+  shows "x \<subseteq># \<Union>#T"
+  using assms
+  using sum_mset.remove by force 
+
+lemma Melem_subset_eq_sum_list [simp]:
+  assumes "x \<in># mset T"
+  shows "x \<subseteq># sum_list T"
+  using assms
+  by (metis mset_subset_eq_add_left sum_mset.remove sum_mset_sum_list)
+
+lemma less_subset_eq_Union_mset[simp]:
+  assumes "i < length CAi"
+  shows "CAi ! i \<subseteq># \<Union>#mset CAi"  
+proof -
+  from assms have "CAi ! i \<in># mset CAi"
+    by auto
+  then show "CAi ! i \<subseteq># \<Union>#mset CAi"
+    by auto
+qed
+
+lemma less_subset_eq_sum_list[simp]:
+  assumes "i < length CAi"
+  shows "CAi ! i \<subseteq># sum_list CAi"  
+proof -
+  from assms have "CAi ! i \<in># mset CAi"
+    by auto
+  then show "CAi ! i \<subseteq># sum_list CAi"
+    by auto
+qed
+
+
 end
